update for Hint Mode +

bedrock2/src/bedrock2/Map/Separation.v
@@ -2,10 +2,10 @@ Require Import coqutil.Map.Interface bedrock2.Lift1Prop. Import map.
 
 Section Sep.
   Context {key value} {map : map key value}.
-  Definition emp (P : Prop) := fun m => m = empty /\ P.
-  Definition sep (p q : rep -> Prop) m :=
+  Definition emp (P : Prop) := fun m : map => m = empty /\ P.
+  Definition sep (p q : map -> Prop) m :=
     exists mp mq, split m mp mq /\ p mp /\ q mq.
-  Definition ptsto k v := fun m => m = put empty k v.
+  Definition ptsto k v := fun m : map => m = put empty k v.
   Definition read k (P : value -> rep -> Prop) := (ex1 (fun v => sep (ptsto k v) (P v))).
 
   Fixpoint seps (xs : list (rep -> Prop)) : rep -> Prop :=
