bedrock2/src/bedrock2/AbsintWordToZ.v
@@ -160,7 +160,7 @@ Module unsigned.
             match reverse goal with H : ?e |- ?G => is_evar e; unify e G; exact H end).. ]
       )) (at level 10, only parsing).
 
-    Lemma absint_of_Z (x : Z) (Hrange : 0 <= x < 2^width) : word.unsigned (word.of_Z x) = x.
+    Lemma absint_of_Z (x : Z) (Hrange : 0 <= x < 2^width) : word.unsigned (word.of_Z (width:=width) x) = x.
     Proof. rewrite word.unsigned_of_Z; unfold word.wrap; rewrite Z.mod_small; trivial. Qed.
     Definition absint_add (x y : word.rep) ux Hx uy Hy Hbounds : _ =~> _ :=
       absint_lemma! (word.unsigned_add x y).
@@ -184,8 +184,9 @@ Module unsigned.
       absint_lemma! (Properties.word.unsigned_divu_nowrap x y).
     Definition absint_modu (x y : word.rep) ux Hx uy Hy Hnz  : word.unsigned _ =~> _ :=
       absint_lemma! (Properties.word.unsigned_modu_nowrap x y).
+    Implicit Types (x y : word).
     (* TODO use it *)
-    Lemma absint_opp (x : word.rep) (ux: Z) (Hx: word.unsigned x = ux) (Hnz: ux <> 0):
+    Lemma absint_opp x (ux: Z) (Hx: word.unsigned x = ux) (Hnz: ux <> 0):
       word.unsigned (word.opp x) =~> 2^width - ux.
     Proof.
       rewrite word.unsigned_opp. cbv [word.wrap].
