compiler/src/compiler/FlattenExpr.v
@@ -467,7 +467,7 @@ Section FlattenExpr1.
     reflexivity.
   Qed.
 
-  Lemma one_ne_zero: word.of_Z 1 <> word.of_Z 0.
+  Lemma one_ne_zero: word.of_Z 1 <> word.of_Z 0 :> word.
   Proof.
     apply unsigned_ne.
     rewrite! word.unsigned_of_Z. unfold word.wrap.
@@ -476,7 +476,7 @@ Section FlattenExpr1.
   Qed.
 
   Lemma bool_to_word_to_bool_id: forall (b: bool),
-      negb (word.eqb (if b then word.of_Z 1 else word.of_Z 0) (word.of_Z 0)) = b.
+      negb (word.eqb (if b then word.of_Z 1 else word.of_Z (width:=width) 0) (word.of_Z 0)) = b.
   Proof.
     intro b. unfold negb.
     destruct_one_match; destruct_one_match_hyp; try reflexivity.
