processor/src/processor/Consistency.v
@@ -88,8 +88,9 @@ Section FetchOk.
   Lemma AddrAligned_plus4:
     forall rpc,
       AddrAligned rpc ->
-      AddrAligned (word.add rpc (word.of_Z 4)).
+      AddrAligned (word.add (width:=width) rpc (word.of_Z 4)).
   Proof.
+    Set Printing Implicit.
     cbv [AddrAligned word.add word WordsKami wordW KamiWord.word].
     intros.
     rewrite <-H.
@@ -341,11 +342,11 @@ Section DecExecOk.
       forall w z,
         Z.of_N (wordToN w) = z ->
         krf w =
-        (if Z.eq_dec z 0 then word.of_Z 0
+        (if Z.eq_dec z 0 then word.of_Z (width:=width) 0
          else
            match map.get rrf z with
            | Some x => x
-           | None => word.of_Z 0
+           | None => word.of_Z (width:=width) 0
            end).
   Proof.
     intros.
